11FlatMemory/MemoryFlattening.thy
@@ -1,19 +1,26 @@
 theory MemoryFlattening                   
-  imports FlatMemory "../09HeapMemory/HeapConversion"
+  imports FlatMemory "../09HeapMemory/HeapConversion" "../10ChainedEnvironment/Chaining"
 begin
 
 primrec flatten_closure :: "ceclosure \<Rightarrow> nat list" where
   "flatten_closure (CEConst k) = [0, k, 0]"
 | "flatten_closure (CELam p pc) = [1, 2 * p, pc]"
 
+primrec flatten_closure' :: "ceclosure \<Rightarrow> ceclosure" where
+  "flatten_closure' (CEConst k) = CEConst k"
+| "flatten_closure' (CELam p pc) = CELam (2 * p) pc"
+
 abbreviation flatten_values :: "ceclosure heap \<Rightarrow> nat heap" where
   "flatten_values h \<equiv> hsplay flatten_closure h"
 
 primrec flatten_env :: "(ptr \<times> ptr) \<Rightarrow> ptr list" where
-  "flatten_env (a, b) = [b, a]"
+  "flatten_env (a, b) = [3 * a, 2 * b]"
 
 abbreviation flatten_environment :: "(ptr \<times> ptr) heap \<Rightarrow> ptr heap" where
   "flatten_environment h \<equiv> hsplay flatten_env h"
+
+abbreviation flatten_vals :: "ptr list \<Rightarrow> ptr list" where
+  "flatten_vals vs \<equiv> map ((*) 3) vs"
 
 primrec flatten_frame :: "(ptr \<times> nat) \<Rightarrow> nat list" where
   "flatten_frame (a, b) = [b, 2 * a]"
@@ -23,50 +30,226 @@ abbreviation flatten_stack :: "(ptr \<times> nat) list \<Rightarrow> nat list" w
 
 primrec flatten :: "chained_state \<Rightarrow> flat_state" where
   "flatten (CES h env vs sfs) = 
-      FS (flatten_values h) (flatten_environment env) vs (flatten_stack sfs)"
+      FS (flatten_values h) (flatten_environment env) (flatten_vals vs) (flatten_stack sfs)"
 
-lemma [simp]: "get_closure (flatten_values h) v = hlookup h v"
-  by simp
+lemma [simp]: "length (flatten_closure c) = 3"
+  by (induction c) simp_all
+
+lemma [simp]: "flatten_closure c ! 0 = (case c of CEConst _ \<Rightarrow> 0 | CELam _ _ \<Rightarrow> 1)"
+  by (simp split: ceclosure.splits)
+
+lemma flatten_c1 [simp]: "flatten_closure c ! 1 = (case c of CEConst k \<Rightarrow> k | CELam p _ \<Rightarrow> 2 * p)"
+  by (simp split: ceclosure.splits)
+
+lemma flatten_c2 [simp]: "flatten_closure c ! 2 = (case c of CEConst k \<Rightarrow> 0 | CELam _ pc \<Rightarrow> pc)"
+  by (simp split: ceclosure.splits)
+
+lemma [simp]: "hcontains h v \<Longrightarrow> 
+  get_closure (flatten_values h) (3 * v) = flatten_closure' (hlookup h v)"
+proof -
+  assume "hcontains h v"
+  hence H: "\<And>k g. (\<And>a. flatten_closure a ! k = g a) \<Longrightarrow>
+    k < 3 \<Longrightarrow> hlookup (hsplay flatten_closure h) (k + 3 * v) = g (hlookup h v)" by simp
+  hence "hlookup (hsplay flatten_closure h) (3 * v) = 
+    (case hlookup h v of CEConst _ \<Rightarrow> 0 | CELam _ _ \<Rightarrow> 1)" by force
+  moreover from H have "hlookup (hsplay flatten_closure h) (Suc (3 * v)) = 
+    (case hlookup h v of CEConst k \<Rightarrow> k | CELam p _ \<Rightarrow> 2 * p)"
+      by (metis flatten_c1 one_less_numeral_iff plus_1_eq_Suc semiring_norm(77))
+  moreover from H have "hlookup (hsplay flatten_closure h) (Suc (Suc (3 * v))) = 
+    (case hlookup h v of CEConst k \<Rightarrow> 0 | CELam _ pc \<Rightarrow> pc)"
+      by (metis flatten_c2 add.left_neutral add_2_eq_Suc' add_Suc eval_nat_numeral(3) lessI)
+  ultimately show ?thesis by (simp split: ceclosure.splits)
+qed
+
+lemma [dest]: "hcontains h v \<Longrightarrow> get_closure (flatten_values h) (3 * v) = CEConst k \<Longrightarrow> 
+    hlookup h v = CEConst k"
+  by (cases "hlookup h v") (simp_all del: get_closure.simps)
+
+lemma [dest]: "hcontains h v \<Longrightarrow> get_closure (flatten_values h) (3 * v) = CELam p pc \<Longrightarrow> 
+    \<exists>p'. hlookup h v = CELam p' pc \<and> p = 2 * p'"
+  by (cases "hlookup h v") (simp_all del: get_closure.simps)
 
 lemma [simp]: "length (flatten_env e) = 2"
   by (induction e) simp_all
 
-lemma [simp]: "fst e = flatten_env e ! 1"
+lemma flatten_e0 [simp]: "(flatten_env e ! 0) = 3 * fst e"
   by (induction e) simp_all
 
-lemma [simp]: "snd e = flatten_env e ! 0"
+lemma flatten_e1 [simp]: "(flatten_env e ! 1) = 2 * snd e"
   by (induction e) simp_all
 
-lemma [simp]: "flat_lookup (flatten_environment env) (2 * p) x = chain_lookup env p x"
-  by (induction env p x rule: chain_lookup.induct) simp_all
+lemma [simp]: "chained_stack_pointer env p \<Longrightarrow> chain_structured h env \<Longrightarrow>
+  flat_lookup (flatten_environment env) (2 * p) x = map_option ((*) 3) (chain_lookup env p x)"
+proof (induction env p x rule: chain_lookup.induct)
+  case (2 env p)
+  hence "hcontains env p" by auto
+  hence "\<And>k g. (\<And>a. flatten_env a ! k = g a) \<Longrightarrow> k < 2 \<Longrightarrow>
+    hlookup (hsplay flatten_env env) (k + 2 * p) = g (hlookup env p)" by simp
+  hence "hlookup (hsplay flatten_env env) (2 * p) = 3 * fst (hlookup env p)" 
+    using flatten_e0 by force
+  thus ?case by (simp split: prod.splits)
+next
+  case (3 env p x)
+  hence P: "hcontains env p" by auto
+  hence "\<And>k g. (\<And>a. flatten_env a ! k = g a) \<Longrightarrow> k < 2 \<Longrightarrow>
+    hlookup (hsplay flatten_env env) (k + 2 * p) = g (hlookup env p)" by simp
+  moreover have "\<And>a. (flatten_env a ! 1) = 2 * snd a \<and> (1::nat) < 2" by auto
+  ultimately have X: "hlookup (hsplay flatten_env env) (1 + 2 * p) = 2 * snd (hlookup env p)" 
+    by meson
+  obtain a b where A: "hlookup env p = (a, b)" by (cases "hlookup env p")
+  with 3 P have "b \<le> p" using heap_lookup_all by fast
+  with P have "chained_stack_pointer env b" by auto
+  with 3 X A show ?case by simp
+qed simp_all
 
 lemma flatten_halloc [simp]: "halloc h c = (h', v) \<Longrightarrow> 
-    halloc_list (flatten_values h) (flatten_closure c) = (flatten_values h', v)"
+    halloc_list (flatten_values h) (flatten_closure c) = (flatten_values h', 3 * v)"
   by simp
 
-theorem correctf: "cd \<tturnstile> flatten \<Sigma>\<^sub>c\<^sub>e \<leadsto>\<^sub>f \<Sigma>\<^sub>f' \<Longrightarrow> \<exists>\<Sigma>\<^sub>c\<^sub>e'. (cd \<tturnstile> \<Sigma>\<^sub>c\<^sub>e \<leadsto>\<^sub>c\<^sub>e \<Sigma>\<^sub>c\<^sub>e') \<and> flatten \<Sigma>\<^sub>c\<^sub>e' = \<Sigma>\<^sub>f'" 
-  by simp
+lemma [dest]: "FS h env vs sfs = flatten \<Sigma>\<^sub>c\<^sub>e \<Longrightarrow> \<exists>h\<^sub>c\<^sub>e env\<^sub>c\<^sub>e vs\<^sub>c\<^sub>e sfs\<^sub>c\<^sub>e. \<Sigma>\<^sub>c\<^sub>e = CES h\<^sub>c\<^sub>e env\<^sub>c\<^sub>e vs\<^sub>c\<^sub>e sfs\<^sub>c\<^sub>e \<and> 
+  h = flatten_values h\<^sub>c\<^sub>e \<and> env = flatten_environment env\<^sub>c\<^sub>e \<and> vs = flatten_vals vs\<^sub>c\<^sub>e \<and> 
+    sfs = flatten_stack sfs\<^sub>c\<^sub>e"
+  by (induction \<Sigma>\<^sub>c\<^sub>e) simp_all
 
-theorem completef [simp]: "cd \<tturnstile> \<Sigma>\<^sub>c\<^sub>e \<leadsto>\<^sub>c\<^sub>e \<Sigma>\<^sub>c\<^sub>e' \<Longrightarrow> cd \<tturnstile> flatten \<Sigma>\<^sub>c\<^sub>e \<leadsto>\<^sub>f flatten \<Sigma>\<^sub>c\<^sub>e'" 
+lemma [dest]: "pc # p # sfs = flatten_stack sfs\<^sub>c\<^sub>e \<Longrightarrow> \<exists>p\<^sub>c\<^sub>e sfs\<^sub>c\<^sub>e'. sfs\<^sub>c\<^sub>e = (p\<^sub>c\<^sub>e, pc) # sfs\<^sub>c\<^sub>e' \<and> 
+  sfs = flatten_stack sfs\<^sub>c\<^sub>e' \<and> p = 2 * p\<^sub>c\<^sub>e"
+proof (induction sfs\<^sub>c\<^sub>e)
+  case (Cons sf\<^sub>c\<^sub>e sfs\<^sub>c\<^sub>e)
+  thus ?case by (cases sf\<^sub>c\<^sub>e) simp_all
+qed simp_all
+
+lemma [dest]: "halloc_list (flatten_values h\<^sub>c\<^sub>e) (flatten_closure c) = (h', v) \<Longrightarrow> 
+  \<exists>h\<^sub>c\<^sub>e' v\<^sub>c\<^sub>e. h' = hsplay flatten_closure h\<^sub>c\<^sub>e' \<and> v = 3 * v\<^sub>c\<^sub>e \<and> halloc h\<^sub>c\<^sub>e c = (h\<^sub>c\<^sub>e', v\<^sub>c\<^sub>e)"
+proof -
+  obtain h\<^sub>c\<^sub>e' v\<^sub>c\<^sub>e where "halloc h\<^sub>c\<^sub>e c = (h\<^sub>c\<^sub>e', v\<^sub>c\<^sub>e)" by fastforce
+  moreover assume "halloc_list (flatten_values h\<^sub>c\<^sub>e) (flatten_closure c) = (h', v)"
+  ultimately show ?thesis by auto
+qed
+
+theorem correctf: "cd \<tturnstile> flatten \<Sigma>\<^sub>c\<^sub>e \<leadsto>\<^sub>f \<Sigma>\<^sub>f' \<Longrightarrow> chained_state \<Sigma>\<^sub>c\<^sub>e \<Longrightarrow> 
+  \<exists>\<Sigma>\<^sub>c\<^sub>e'. (cd \<tturnstile> \<Sigma>\<^sub>c\<^sub>e \<leadsto>\<^sub>c\<^sub>e \<Sigma>\<^sub>c\<^sub>e') \<and> flatten \<Sigma>\<^sub>c\<^sub>e' = \<Sigma>\<^sub>f'" 
+proof (induction "flatten \<Sigma>\<^sub>c\<^sub>e" \<Sigma>\<^sub>f' rule: evalf.induct)
+  case (evf_lookup cd pc x env p v h vs sfs)
+  then obtain h\<^sub>c\<^sub>e env\<^sub>c\<^sub>e vs\<^sub>c\<^sub>e p\<^sub>c\<^sub>e sfs\<^sub>c\<^sub>e where S: "\<Sigma>\<^sub>c\<^sub>e = CES h\<^sub>c\<^sub>e env\<^sub>c\<^sub>e vs\<^sub>c\<^sub>e ((p\<^sub>c\<^sub>e, Suc pc) # sfs\<^sub>c\<^sub>e) \<and> 
+    h = flatten_values h\<^sub>c\<^sub>e \<and> env = flatten_environment env\<^sub>c\<^sub>e \<and> vs = flatten_vals vs\<^sub>c\<^sub>e \<and> 
+      sfs = flatten_stack sfs\<^sub>c\<^sub>e \<and> p = 2 * p\<^sub>c\<^sub>e" by fastforce
+  with evf_lookup obtain v\<^sub>c\<^sub>e where V: "chain_lookup env\<^sub>c\<^sub>e p\<^sub>c\<^sub>e x = Some v\<^sub>c\<^sub>e \<and> v = 3 * v\<^sub>c\<^sub>e" by fastforce
+  with S have X: "flatten (CES h\<^sub>c\<^sub>e env\<^sub>c\<^sub>e (v\<^sub>c\<^sub>e # vs\<^sub>c\<^sub>e) ((p\<^sub>c\<^sub>e, pc) # sfs\<^sub>c\<^sub>e)) = 
+    FS h env (v # vs) (pc # p # sfs)" by simp
+  from evf_lookup V have "cd \<tturnstile> CES h\<^sub>c\<^sub>e env\<^sub>c\<^sub>e vs\<^sub>c\<^sub>e ((p\<^sub>c\<^sub>e, Suc pc) # sfs\<^sub>c\<^sub>e) \<leadsto>\<^sub>c\<^sub>e 
+    CES h\<^sub>c\<^sub>e env\<^sub>c\<^sub>e (v\<^sub>c\<^sub>e # vs\<^sub>c\<^sub>e) ((p\<^sub>c\<^sub>e, pc) # sfs\<^sub>c\<^sub>e)" by simp
+  with S X show ?case by blast
+next
+  case (evf_pushcon cd pc k h h' v env vs p sfs)
+  then obtain h\<^sub>c\<^sub>e env\<^sub>c\<^sub>e vs\<^sub>c\<^sub>e p\<^sub>c\<^sub>e sfs\<^sub>c\<^sub>e where S: "\<Sigma>\<^sub>c\<^sub>e = CES h\<^sub>c\<^sub>e env\<^sub>c\<^sub>e vs\<^sub>c\<^sub>e ((p\<^sub>c\<^sub>e, Suc pc) # sfs\<^sub>c\<^sub>e) \<and> 
+    h = flatten_values h\<^sub>c\<^sub>e \<and> env = flatten_environment env\<^sub>c\<^sub>e \<and> vs = flatten_vals vs\<^sub>c\<^sub>e \<and> 
+      sfs = flatten_stack sfs\<^sub>c\<^sub>e \<and> p = 2 * p\<^sub>c\<^sub>e" by fastforce
+  with evf_pushcon have "halloc_list (hsplay flatten_closure h\<^sub>c\<^sub>e) (flatten_closure (CEConst k)) = 
+    (h', v)" by simp
+  then obtain h\<^sub>c\<^sub>e' v\<^sub>c\<^sub>e where H: "h' = hsplay flatten_closure h\<^sub>c\<^sub>e' \<and> v = 3 * v\<^sub>c\<^sub>e \<and> 
+    halloc h\<^sub>c\<^sub>e (CEConst k) = (h\<^sub>c\<^sub>e', v\<^sub>c\<^sub>e)" by fastforce
+  with S have X: "flatten (CES h\<^sub>c\<^sub>e' env\<^sub>c\<^sub>e (v\<^sub>c\<^sub>e # vs\<^sub>c\<^sub>e) ((p\<^sub>c\<^sub>e, pc) # sfs\<^sub>c\<^sub>e)) = 
+    FS h' env (v # vs) (pc # p # sfs)" by simp
+  from evf_pushcon H have "cd \<tturnstile> CES h\<^sub>c\<^sub>e env\<^sub>c\<^sub>e vs\<^sub>c\<^sub>e ((p\<^sub>c\<^sub>e, Suc pc) # sfs\<^sub>c\<^sub>e) \<leadsto>\<^sub>c\<^sub>e 
+    CES h\<^sub>c\<^sub>e' env\<^sub>c\<^sub>e (v\<^sub>c\<^sub>e # vs\<^sub>c\<^sub>e) ((p\<^sub>c\<^sub>e, pc) # sfs\<^sub>c\<^sub>e)" by simp
+  with S X show ?case by blast
+next
+  case (evf_pushlam cd pc pc' h p h' v env vs sfs)
+  then obtain h\<^sub>c\<^sub>e env\<^sub>c\<^sub>e vs\<^sub>c\<^sub>e p\<^sub>c\<^sub>e sfs\<^sub>c\<^sub>e where S: "\<Sigma>\<^sub>c\<^sub>e = CES h\<^sub>c\<^sub>e env\<^sub>c\<^sub>e vs\<^sub>c\<^sub>e ((p\<^sub>c\<^sub>e, Suc pc) # sfs\<^sub>c\<^sub>e) \<and> 
+    h = flatten_values h\<^sub>c\<^sub>e \<and> env = flatten_environment env\<^sub>c\<^sub>e \<and> vs = flatten_vals vs\<^sub>c\<^sub>e \<and> 
+      sfs = flatten_stack sfs\<^sub>c\<^sub>e \<and> p = 2 * p\<^sub>c\<^sub>e" by fastforce
+  with evf_pushlam have "halloc_list (hsplay flatten_closure h\<^sub>c\<^sub>e) (flatten_closure (CELam p\<^sub>c\<^sub>e pc')) = 
+    (h', v)" by simp
+  then obtain h\<^sub>c\<^sub>e' v\<^sub>c\<^sub>e where H: "h' = hsplay flatten_closure h\<^sub>c\<^sub>e' \<and> v = 3 * v\<^sub>c\<^sub>e \<and> 
+    halloc h\<^sub>c\<^sub>e (CELam p\<^sub>c\<^sub>e pc') = (h\<^sub>c\<^sub>e', v\<^sub>c\<^sub>e)" by fastforce
+  with S have X: "flatten (CES h\<^sub>c\<^sub>e' env\<^sub>c\<^sub>e (v\<^sub>c\<^sub>e # vs\<^sub>c\<^sub>e) ((p\<^sub>c\<^sub>e, pc) # sfs\<^sub>c\<^sub>e)) = 
+    FS h' env (v # vs) (pc # p # sfs)" by simp
+  from evf_pushlam S H have "cd \<tturnstile> CES h\<^sub>c\<^sub>e env\<^sub>c\<^sub>e vs\<^sub>c\<^sub>e ((p\<^sub>c\<^sub>e, Suc pc) # sfs\<^sub>c\<^sub>e) \<leadsto>\<^sub>c\<^sub>e 
+    CES h\<^sub>c\<^sub>e' env\<^sub>c\<^sub>e (v\<^sub>c\<^sub>e # vs\<^sub>c\<^sub>e) ((p\<^sub>c\<^sub>e, pc) # sfs\<^sub>c\<^sub>e)" by simp
+  with S X show ?case by blast
+next
+  case (evf_apply cd pc h v2 p' pc' env v1 env' p2 vs p sfs)
+  then obtain h\<^sub>c\<^sub>e env\<^sub>c\<^sub>e v1\<^sub>c\<^sub>e v2\<^sub>c\<^sub>e vs\<^sub>c\<^sub>e p\<^sub>c\<^sub>e sfs\<^sub>c\<^sub>e where S: "
+    \<Sigma>\<^sub>c\<^sub>e = CES h\<^sub>c\<^sub>e env\<^sub>c\<^sub>e (v1\<^sub>c\<^sub>e # v2\<^sub>c\<^sub>e # vs\<^sub>c\<^sub>e) ((p\<^sub>c\<^sub>e, Suc pc) # sfs\<^sub>c\<^sub>e) \<and> h = flatten_values h\<^sub>c\<^sub>e \<and> 
+      env = flatten_environment env\<^sub>c\<^sub>e \<and> v1 = 3 * v1\<^sub>c\<^sub>e \<and> v2 = 3 * v2\<^sub>c\<^sub>e \<and> vs = flatten_vals vs\<^sub>c\<^sub>e \<and> 
+        sfs = flatten_stack sfs\<^sub>c\<^sub>e \<and> p = 2 * p\<^sub>c\<^sub>e" by fastforce
+  with evf_apply have "get_closure (flatten_values h\<^sub>c\<^sub>e) (3 * v2\<^sub>c\<^sub>e) = CELam p' pc'" by simp
+  moreover from evf_apply S have "hcontains h\<^sub>c\<^sub>e v2\<^sub>c\<^sub>e" by simp
+  ultimately obtain p\<^sub>c\<^sub>e' where P: "hlookup h\<^sub>c\<^sub>e v2\<^sub>c\<^sub>e = CELam p\<^sub>c\<^sub>e' pc' \<and> p' = 2 * p\<^sub>c\<^sub>e'" by blast
+
+
+  have "halloc env\<^sub>c\<^sub>e a = (env\<^sub>c\<^sub>e', p2\<^sub>c\<^sub>e) \<Longrightarrow> 
+  halloc_list (flatten_environment env\<^sub>c\<^sub>e) (flatten_env a) = (flatten_environment env\<^sub>c\<^sub>e', 2 * p2\<^sub>c\<^sub>e)" by simp
+
+  from evf_apply S P have "halloc_list (flatten_environment env\<^sub>c\<^sub>e) (flatten_env (v1\<^sub>c\<^sub>e, p\<^sub>c\<^sub>e')) = (env', p2)" by simp
+
+  from S P have X: "flatten (CES h\<^sub>c\<^sub>e env\<^sub>c\<^sub>e' vs\<^sub>c\<^sub>e ((Suc xp\<^sub>c\<^sub>e', pc') # (p\<^sub>c\<^sub>e, pc) # sfs\<^sub>c\<^sub>e)) = 
+    FS h env' vs (pc' # Suc (Suc p2) # pc # p # sfs)" by simp
+
+
+  have "halloc env\<^sub>c\<^sub>e (v1\<^sub>c\<^sub>e, p\<^sub>c\<^sub>e') = (env\<^sub>c\<^sub>e', xp\<^sub>c\<^sub>e')" by simp
+  with evf_apply P have "cd \<tturnstile> CES h\<^sub>c\<^sub>e env\<^sub>c\<^sub>e (v1\<^sub>c\<^sub>e # v2\<^sub>c\<^sub>e # vs\<^sub>c\<^sub>e) ((p\<^sub>c\<^sub>e, Suc pc) # sfs\<^sub>c\<^sub>e) \<leadsto>\<^sub>c\<^sub>e 
+        CES h\<^sub>c\<^sub>e env\<^sub>c\<^sub>e' vs\<^sub>c\<^sub>e ((Suc xp\<^sub>c\<^sub>e', pc') # (p\<^sub>c\<^sub>e, pc) # sfs\<^sub>c\<^sub>e)" by simp
+  with S X show ?case by blast
+next
+  case (evf_return cd pc h env vs p sfs)
+  then obtain h\<^sub>c\<^sub>e env\<^sub>c\<^sub>e vs\<^sub>c\<^sub>e p\<^sub>c\<^sub>e sfs\<^sub>c\<^sub>e where S: "\<Sigma>\<^sub>c\<^sub>e = CES h\<^sub>c\<^sub>e env\<^sub>c\<^sub>e vs\<^sub>c\<^sub>e ((p\<^sub>c\<^sub>e, Suc pc) # sfs\<^sub>c\<^sub>e) \<and> 
+    h = flatten_values h\<^sub>c\<^sub>e \<and> env = flatten_environment env\<^sub>c\<^sub>e \<and> vs = flatten_vals vs\<^sub>c\<^sub>e \<and> 
+      sfs = flatten_stack sfs\<^sub>c\<^sub>e \<and> p = 2 * p\<^sub>c\<^sub>e" by fastforce
+
+  then show ?case by simp
+next
+  case (evf_jump cd pc h v2 p' pc' env v1 env' p2 vs p sfs)
+  then obtain h\<^sub>c\<^sub>e env\<^sub>c\<^sub>e v1\<^sub>c\<^sub>e v2\<^sub>c\<^sub>e vs\<^sub>c\<^sub>e p\<^sub>c\<^sub>e sfs\<^sub>c\<^sub>e where S: "
+    \<Sigma>\<^sub>c\<^sub>e = CES h\<^sub>c\<^sub>e env\<^sub>c\<^sub>e (v1\<^sub>c\<^sub>e # v2\<^sub>c\<^sub>e # vs\<^sub>c\<^sub>e) ((p\<^sub>c\<^sub>e, Suc pc) # sfs\<^sub>c\<^sub>e) \<and> h = flatten_values h\<^sub>c\<^sub>e \<and> 
+      env = flatten_environment env\<^sub>c\<^sub>e \<and> v1 = 3 * v1\<^sub>c\<^sub>e \<and> v2 = 3 * v2\<^sub>c\<^sub>e \<and> vs = flatten_vals vs\<^sub>c\<^sub>e \<and> 
+        sfs = flatten_stack sfs\<^sub>c\<^sub>e \<and> p = 2 * p\<^sub>c\<^sub>e" by fastforce
+
+  then show ?case by simp
+qed
+
+theorem completef [simp]: "cd \<tturnstile> \<Sigma>\<^sub>c\<^sub>e \<leadsto>\<^sub>c\<^sub>e \<Sigma>\<^sub>c\<^sub>e' \<Longrightarrow> chained_state \<Sigma>\<^sub>c\<^sub>e \<Longrightarrow> 
+  cd \<tturnstile> flatten \<Sigma>\<^sub>c\<^sub>e \<leadsto>\<^sub>f flatten \<Sigma>\<^sub>c\<^sub>e'" 
 proof (induction \<Sigma>\<^sub>c\<^sub>e \<Sigma>\<^sub>c\<^sub>e' rule: evalce.induct)
+  case (evce_lookup cd pc x env p v h vs sfs)
+  hence "chain_structured h env \<and> chained_closures env h \<and> chained_vals h vs \<and> chained_frame env (p, Suc pc) \<and> chained_stack env sfs" by simp
+
+  from evce_lookup have "hcontains env p \<Longrightarrow>
+    flat_lookup (flatten_environment env) (2 * p) x = map_option ((*) 3) (chain_lookup env p x)" by simp
+
+  have "cd \<tturnstile> FS (flatten_values h) (flatten_environment env) (flatten_vals vs) 
+    (Suc pc # 2 * p # flatten_stack sfs) \<leadsto>\<^sub>f
+      FS (flatten_values h) (flatten_environment env) (3 * v # flatten_vals vs) 
+        (pc # 2 * p # flatten_stack sfs)" by simp
+  then show ?case by simp
+next
   case (evce_pushcon cd pc k h h' v env vs p sfs)
-  moreover hence "halloc_list (flatten_values h) [0, k, 0] = (flatten_values h', v)" 
+  moreover hence "halloc_list (flatten_values h) [0, k, 0] = (flatten_values h', 3 * v)"
     using flatten_halloc by fastforce
   ultimately show ?case by simp
 next
   case (evce_pushlam cd pc pc' h p h' v env vs sfs)
-  moreover hence "halloc_list (flatten_values h) [1, 2 * p, pc'] = (flatten_values h', v)" 
+  moreover hence "halloc_list (flatten_values h) [1, 2 * p, pc'] = (flatten_values h', 3 * v)" 
     using flatten_halloc by fastforce
   ultimately show ?case by simp
 next
   case (evce_apply cd pc h v2 p' pc' env v1 env' p'' vs p sfs)
+  from evce_apply have "cd ! pc = BApply" by simp
+  from evce_apply have "hlookup h v2 = CELam p' pc'" by simp
+  from evce_apply have "halloc env (v1, p') = (env', p'')" by simp
+
+
+  have "cd \<tturnstile> FS (flatten_values h) (flatten_environment env) (3 * v1 # 3 * v2 # flatten_vals vs) 
+    (Suc pc # 2 * p # flatten_stack sfs) \<leadsto>\<^sub>f
+      FS (flatten_values h) (flatten_environment env') (flatten_vals vs) 
+        (pc' # Suc (Suc (2 * p'')) # pc # 2 * p # flatten_stack sfs)" by simp
   then show ?case by simp
 next
   case (evce_jump cd pc h v2 p' pc' env v1 env' p'' vs p sfs)
   then show ?case by simp
 qed simp_all
 
-lemma completef_iter [simp]: "iter (\<tturnstile> cd \<leadsto>\<^sub>c\<^sub>e) \<Sigma>\<^sub>c\<^sub>e \<Sigma>\<^sub>c\<^sub>e' \<Longrightarrow> 
+lemma completef_iter [simp]: "iter (\<tturnstile> cd \<leadsto>\<^sub>c\<^sub>e) \<Sigma>\<^sub>c\<^sub>e \<Sigma>\<^sub>c\<^sub>e' \<Longrightarrow> chained_state \<Sigma>\<^sub>c\<^sub>e \<Longrightarrow>
   iter (\<tturnstile> cd \<leadsto>\<^sub>f) (flatten \<Sigma>\<^sub>c\<^sub>e) (flatten \<Sigma>\<^sub>c\<^sub>e')"
 proof (induction \<Sigma>\<^sub>c\<^sub>e \<Sigma>\<^sub>c\<^sub>e' rule: iter.induct)
   case (iter_step \<Sigma>\<^sub>c\<^sub>e \<Sigma>\<^sub>c\<^sub>e' \<Sigma>\<^sub>c\<^sub>e'')
