12UnstructuredMemory/UnstructuredMemory.thy
@@ -4,6 +4,7 @@ begin
 
 datatype unstr_state = 
   US "nat \<Rightarrow> nat" nat "nat \<Rightarrow> nat" nat "nat \<Rightarrow> nat" nat "nat \<Rightarrow> nat" nat nat
+  | USF "nat \<Rightarrow> nat" nat "nat \<Rightarrow> nat" nat "nat \<Rightarrow> nat" nat
 
 fun unstr_lookup :: "(nat \<Rightarrow> nat) \<Rightarrow> nat \<Rightarrow> nat \<rightharpoonup> nat" where
   "unstr_lookup h 0 x = None"
@@ -12,7 +13,7 @@ fun unstr_lookup :: "(nat \<Rightarrow> nat) \<Rightarrow> nat \<Rightarrow> nat
 | "unstr_lookup h (Suc (Suc p)) (Suc x) = unstr_lookup h (h (Suc p)) x"
 
 inductive evalu :: "byte_code list \<Rightarrow> unstr_state \<Rightarrow> unstr_state \<Rightarrow> bool" (infix "\<tturnstile> _ \<leadsto>\<^sub>u" 50) where
-  evu_lookup [simp]: "cd ! pc = BLookup x \<Longrightarrow> unstr_lookup h (sh (sp - 1)) (Suc x) = Some y \<Longrightarrow>
+  evu_lookup [simp]: "cd ! pc = BLookup x \<Longrightarrow> unstr_lookup e (sh (sp - 1)) x = Some y \<Longrightarrow>
     cd \<tturnstile> US h hp e ep vs vp sh sp (Suc pc) \<leadsto>\<^sub>u US h hp e ep (vs(vp := y)) (Suc vp) sh sp pc"
 | evu_pushcon [simp]: "cd ! pc = BPushCon k \<Longrightarrow> 
     cd \<tturnstile> US h hp e ep vs vp sh sp (Suc pc) \<leadsto>\<^sub>u 
@@ -20,22 +21,24 @@ inductive evalu :: "byte_code list \<Rightarrow> unstr_state \<Rightarrow> unstr
         (vs(vp := hp)) (Suc vp) sh sp pc"
 | evu_pushlam [simp]: "cd ! pc = BPushLam pc' \<Longrightarrow> 
     cd \<tturnstile> US h hp e ep vs vp sh sp (Suc pc) \<leadsto>\<^sub>u 
-      US (h(hp := 1, Suc hp := (sh (sp - 1)), Suc (Suc hp) := pc')) (3 + hp) e ep 
+      US (h(hp := 1, Suc hp := sh (sp - 1), Suc (Suc hp) := pc')) (3 + hp) e ep 
         (vs(vp := hp)) (Suc vp) sh sp pc"
-| evu_apply [simp]: "cd ! pc = BApply \<Longrightarrow> h (vs (vp - 2)) = 1 \<Longrightarrow> 
-    cd \<tturnstile> US h hp e ep vs vp sh sp (Suc pc) \<leadsto>\<^sub>u 
-      US h hp (e(ep := vs (vp - 1), Suc ep := h (Suc (vs (vp - 2))))) (2 + ep) vs (vp - 2) 
-        (sh(sp := Suc (Suc ep), Suc sp := h (Suc (Suc (vs (vp - 2)))))) (2 + sp) pc"
-| evu_return [simp]: "cd ! pc = BReturn \<Longrightarrow> 
-    cd \<tturnstile> US h hp e ep vs vp sh sp (Suc pc) \<leadsto>\<^sub>u US h hp e ep vs vp sh (sp - 1) (sh(sp - 1))"
-| evu_jump [simp]: "cd ! pc = BJump \<Longrightarrow> h (vs (vp - 2)) = 1 \<Longrightarrow> 
-    cd \<tturnstile> US h hp e ep vs vp sh sp (Suc pc) \<leadsto>\<^sub>u 
-      US h hp (e(ep := vs (vp - 1), Suc ep := h (Suc (vs (vp - 2))))) (2 + ep) vs (vp - 2) 
-        (sh(sp - 2 := Suc (Suc ep), sp - 1 := h (Suc (Suc (vs (vp - 2)))))) sp pc"
+| evu_apply [simp]: "cd ! pc = BApply \<Longrightarrow> h (vs vp) = 1 \<Longrightarrow> 
+    cd \<tturnstile> US h hp e ep vs (Suc (Suc vp)) sh sp (Suc pc) \<leadsto>\<^sub>u 
+      US h hp (e(ep := vs (Suc vp), Suc ep := h (Suc (vs vp)))) (2 + ep) vs vp
+        (sh(sp := pc, Suc sp := Suc (Suc ep))) (2 + sp) (h (Suc (Suc (vs vp))))"
+| evu_return_normal [simp]: "cd ! pc = BReturn \<Longrightarrow> 
+    cd \<tturnstile> US h hp e ep vs vp sh (Suc (Suc sp)) (Suc pc) \<leadsto>\<^sub>u US h hp e ep vs vp sh sp (sh sp)"
+| evu_return_end [simp]: "cd ! pc = BReturn \<Longrightarrow> 
+    cd \<tturnstile> US h hp e ep vs vp sh (Suc 0) (Suc pc) \<leadsto>\<^sub>u USF h hp e ep vs vp"
+| evu_jump [simp]: "cd ! pc = BJump \<Longrightarrow> h (vs vp) = 1 \<Longrightarrow> 
+    cd \<tturnstile> US h hp e ep vs (Suc (Suc vp)) sh (Suc (Suc sp)) (Suc pc) \<leadsto>\<^sub>u 
+      US h hp (e(ep := vs (Suc vp), Suc ep := h (Suc (vs vp)))) (2 + ep) vs vp
+        (sh(sp := sh sp, Suc sp := Suc (Suc ep))) (2 + sp) (h (Suc (Suc (vs vp))))"
 
 theorem determinismu: "cd \<tturnstile> \<Sigma> \<leadsto>\<^sub>u \<Sigma>' \<Longrightarrow> cd \<tturnstile> \<Sigma> \<leadsto>\<^sub>u \<Sigma>'' \<Longrightarrow> \<Sigma>' = \<Sigma>''"
 proof (induction cd \<Sigma> \<Sigma>' rule: evalu.induct)
-  case (evu_lookup cd pc x h sh sp y hp e ep vs vp)
+  case (evu_lookup cd pc x e sh sp y h hp ep vs vp)
   from evu_lookup(3, 1, 2) show ?case 
     by (induction cd "US h hp e ep vs vp sh sp (Suc pc)" \<Sigma>'' rule: evalu.induct) simp_all
 next
@@ -50,15 +53,23 @@ next
 next
   case (evu_apply cd pc h vs vp hp e ep sh sp)
   from evu_apply(3, 1, 2) show ?case    
-    by (induction cd "US h hp e ep vs vp sh sp (Suc pc)" \<Sigma>'' rule: evalu.induct) simp_all
+    by (induction cd "US h hp e ep vs (Suc (Suc vp)) sh sp (Suc pc)" \<Sigma>'' rule: evalu.induct) 
+       simp_all
 next
-  case (evu_return cd pc h hp e ep vs vp sh sp)
-  from evu_return(2, 1) show ?case 
-    by (induction cd "US h hp e ep vs vp sh sp (Suc pc)" \<Sigma>'' rule: evalu.induct) simp_all
+  case (evu_return_normal cd pc h hp e ep vs vp sh sp)
+  from evu_return_normal(2, 1) show ?case 
+    by (induction cd "US h hp e ep vs vp sh (Suc (Suc sp)) (Suc pc)" \<Sigma>'' rule: evalu.induct) 
+       simp_all
+next
+  case (evu_return_end cd pc h hp e ep vs vp sh)
+  from evu_return_end(2, 1) show ?case 
+    by (induction cd "US h hp e ep vs vp sh (Suc 0) (Suc pc)" \<Sigma>'' rule: evalu.induct) simp_all
 next
   case (evu_jump cd pc h vs vp hp e ep sh sp)
   from evu_jump(3, 1, 2) show ?case    
-    by (induction cd "US h hp e ep vs vp sh sp (Suc pc)" \<Sigma>'' rule: evalu.induct) simp_all
+    by (induction cd "US h hp e ep vs (Suc (Suc vp)) sh (Suc (Suc sp)) (Suc pc)" \<Sigma>'' 
+        rule: evalu.induct) 
+       simp_all
 qed
 
 end
