12UnstructuredMemory/Unstructuring.thy
@@ -2,77 +2,98 @@ theory Unstructuring
   imports UnstructuredMemory "../11FlatMemory/FlatMemory" "../00Utils/Utils"
 begin
 
-fun restructure :: "unstr_state \<Rightarrow> flat_state" where
-  "restructure (US h hp e ep vs vp sh sp 0) = 
+primrec restructure :: "unstr_state \<Rightarrow> flat_state" where
+  "restructure (US h hp e ep vs vp sh sp pc) = 
+    FS (H h hp) (H e ep) (listify' vs vp) (pc # listify' sh sp)"
+| "restructure (USF h hp e ep vs vp) = 
     FS (H h hp) (H e ep) (listify' vs vp) []"
-| "restructure (US h hp e ep vs vp sh sp (Suc pc)) = 
-    FS (H h hp) (H e ep) (listify' vs vp) (Suc pc # listify' sh sp)"
 
-theorem completeu [simp]: "cd \<tturnstile> \<Sigma>\<^sub>u \<leadsto>\<^sub>u \<Sigma>\<^sub>u' \<Longrightarrow> cd \<tturnstile> restructure \<Sigma>\<^sub>u \<leadsto>\<^sub>f restructure \<Sigma>\<^sub>u'"
-proof (induction \<Sigma>\<^sub>u \<Sigma>\<^sub>u' rule: evalu.induct)
-  case (evu_lookup cd pc x h sh sp y hp e ep vs vp)
-  then show ?case by simp
-next
-  case (evu_pushcon cd pc k h hp e ep vs vp sh sp)
-  then show ?case by simp
-next
-  case (evu_pushlam cd pc pc' h hp e ep vs vp sh sp)
-  then show ?case by simp
-next
-  case (evu_apply cd pc h vs vp hp e ep sh sp)
-  then show ?case by simp
-next
-  case (evu_return cd pc h hp e ep vs vp sh sp)
-  then show ?case by simp
-next
-  case (evu_jump cd pc h vs vp hp e ep sh sp)
-  then show ?case by simp
-qed
+primrec restructurable :: "unstr_state \<Rightarrow> bool" where
+  "restructurable (US h hp e ep vs vp sh sp pc) = (\<exists>sp'. sp = Suc (2 * sp'))"
+| "restructurable (USF h hp e ep vs vp) = True"
 
-lemma [simp]: "iter (\<tturnstile> cd \<leadsto>\<^sub>u) \<Sigma>\<^sub>u \<Sigma>\<^sub>u' \<Longrightarrow> iter (\<tturnstile> cd \<leadsto>\<^sub>f) (restructure \<Sigma>\<^sub>u) (restructure \<Sigma>\<^sub>u')" 
-  by (induction \<Sigma>\<^sub>u \<Sigma>\<^sub>u' rule: iter.induct) (simp, metis completeu iter_step)
+lemma preserve_restructure [simp]: "cd \<tturnstile> \<Sigma>\<^sub>u \<leadsto>\<^sub>u \<Sigma>\<^sub>u' \<Longrightarrow> restructurable \<Sigma>\<^sub>u \<Longrightarrow> restructurable \<Sigma>\<^sub>u'"
+  by (induction \<Sigma>\<^sub>u \<Sigma>\<^sub>u' rule: evalu.induct) (auto, presburger+)
 
-lemma evalu_clears_regs: "iter (\<tturnstile> cd \<leadsto>\<^sub>u) (US nmem 0 nmem 0 nmem 0 (nmem(0 := 0)) 1 (length cd)) 
-    (US h\<^sub>u hp\<^sub>u e\<^sub>u ep\<^sub>u vs\<^sub>u 1 sh\<^sub>u sp\<^sub>u 0) \<Longrightarrow> sp\<^sub>u = 0"
-  by simp
+lemma [simp]: "flat_lookup (H h hp) p x = unstr_lookup h p x"
+  by (induction h p x rule: unstr_lookup.induct) simp_all
 
-lemma [dest]: "FS h env vs sfs = restructure \<Sigma> \<Longrightarrow> \<exists>h' hp e ep vs' vp sh sp pc. 
-  \<Sigma> = US h' hp e ep vs' vp sh sp pc \<and> h = H h' hp \<and> env = H e ep \<and> vs = listify' vs' vp \<and> 
-    ((pc = 0 \<and> sfs = []) \<or> (\<exists>pc'. pc = Suc pc' \<and> sfs = pc # listify' sh sp))"
-  by (induction \<Sigma> rule: restructure.induct) simp_all
+theorem completeu [simp]: "cd \<tturnstile> \<Sigma>\<^sub>u \<leadsto>\<^sub>u \<Sigma>\<^sub>u' \<Longrightarrow> restructurable \<Sigma>\<^sub>u \<Longrightarrow> 
+    cd \<tturnstile> restructure \<Sigma>\<^sub>u \<leadsto>\<^sub>f restructure \<Sigma>\<^sub>u'"
+  by (induction \<Sigma>\<^sub>u \<Sigma>\<^sub>u' rule: evalu.induct) fastforce+
+
+lemma [simp]: "iter (\<tturnstile> cd \<leadsto>\<^sub>u) \<Sigma>\<^sub>u \<Sigma>\<^sub>u' \<Longrightarrow> restructurable \<Sigma>\<^sub>u \<Longrightarrow> 
+    iter (\<tturnstile> cd \<leadsto>\<^sub>f) (restructure \<Sigma>\<^sub>u) (restructure \<Sigma>\<^sub>u')" 
+  by (induction \<Sigma>\<^sub>u \<Sigma>\<^sub>u' rule: iter.induct) (simp, metis completeu iter_step preserve_restructure)
+
+lemma [dest]: "FS h env vs (pc # p # sfs) = restructure \<Sigma> \<Longrightarrow> \<exists>h' hp e ep vs' vp sh sp. 
+  \<Sigma> = US h' hp e ep vs' vp sh (Suc sp) pc \<and> h = H h' hp \<and> env = H e ep \<and> vs = listify' vs' vp \<and> 
+    p = sh sp \<and> sfs = listify' sh sp"
+proof (induction \<Sigma>)
+  case (US h' hp e ep vs' vp sh sp pc')
+  thus ?case by (cases sp) simp_all
+qed simp_all
 
 theorem correctu [simp]: "cd \<tturnstile> restructure \<Sigma>\<^sub>u \<leadsto>\<^sub>f \<Sigma>\<^sub>f' \<Longrightarrow> 
     \<exists>\<Sigma>\<^sub>u'. (cd \<tturnstile> \<Sigma>\<^sub>u \<leadsto>\<^sub>u \<Sigma>\<^sub>u') \<and> \<Sigma>\<^sub>f' = restructure \<Sigma>\<^sub>u'"
 proof (induction "restructure \<Sigma>\<^sub>u" \<Sigma>\<^sub>f' rule: evalf.induct)
   case (evf_lookup cd pc x env p v h vs sfs)
-  hence "FS h env vs (Suc pc # p # sfs) = restructure \<Sigma>\<^sub>u" by simp
-  then obtain h' hp e ep vs' vp sh sp where S: "
-    \<Sigma>\<^sub>u = US h' hp e ep vs' vp sh sp (Suc pc) \<and> h = H h' hp \<and> env = H e ep \<and> 
-      vs = listify' vs' vp \<and> p # sfs = listify' sh sp" by fastforce
-
-
-  from evf_lookup have "cd ! pc = BLookup x" by simp
-  from evf_lookup have "flat_lookup env p x = Some v" by simp
-
-
-
-  from S have "(cd \<tturnstile> US h' hp e ep vs' vp sh sp (Suc pc) \<leadsto>\<^sub>u US h' hp e ep xvs xvp sh sp (Suc xpc)) \<and> 
-    FS h env (v # vs) (pc # p # sfs) = restructure (US h' hp e ep xvs xvp sh sp (Suc xpc))" by simp
-  with S show ?case by blast
+  then obtain h' hp e ep vs' vp sh sp where S: "\<Sigma>\<^sub>u = US h' hp e ep vs' vp sh (Suc sp) (Suc pc) \<and> 
+    h = H h' hp \<and> env = H e ep \<and> vs = listify' vs' vp \<and> p = sh sp \<and> sfs = listify' sh sp" 
+      by fastforce
+  moreover hence "FS h env (v # vs) (pc # p # sfs) = 
+    restructure (US h' hp e ep (vs'(vp := v)) (Suc vp) sh (Suc sp) pc)" by simp
+  moreover from evf_lookup S have "cd \<tturnstile> US h' hp e ep vs' vp sh (Suc sp) (Suc pc) \<leadsto>\<^sub>u 
+    US h' hp e ep (vs'(vp := v)) (Suc vp) sh (Suc sp) pc" by simp
+  ultimately show ?case by blast
 next
   case (evf_pushcon cd pc k h h' v env vs p sfs)
-  then show ?case by simp
+  then obtain hh hp e ep vs' vp sh sp where S: "\<Sigma>\<^sub>u = US hh hp e ep vs' vp sh (Suc sp) (Suc pc) \<and> 
+    h = H hh hp \<and> env = H e ep \<and> vs = listify' vs' vp \<and> p = sh sp \<and> sfs = listify' sh sp" 
+      by fastforce
+  with evf_pushcon have "v = hp \<and> 
+    h' = H (hh(hp := 0, Suc hp := k, Suc (Suc hp) := 0)) (Suc (Suc (Suc hp)))" by fastforce
+  with S have X: "FS h' env (v # vs) (pc # p # sfs) = 
+    restructure (US (hh(hp := 0, Suc hp := k, Suc (Suc hp) := 0)) (3 + hp) e ep 
+      (vs'(vp := hp)) (Suc vp) sh (Suc sp) pc)" by simp
+  from evf_pushcon have "cd \<tturnstile> US hh hp e ep vs' vp sh (Suc sp) (Suc pc) \<leadsto>\<^sub>u 
+    US (hh(hp := 0, Suc hp := k, Suc (Suc hp) := 0)) (3 + hp) e ep (vs'(vp := hp)) 
+      (Suc vp) sh (Suc sp) pc" by simp
+  with S X show ?case by blast
 next
   case (evf_pushlam cd pc pc' h p h' v env vs sfs)
-  then show ?case by simp
+  then obtain hh hp e ep vs' vp sh sp where S: "\<Sigma>\<^sub>u = US hh hp e ep vs' vp sh (Suc sp) (Suc pc) \<and> 
+    h = H hh hp \<and> env = H e ep \<and> vs = listify' vs' vp \<and> p = sh sp \<and> sfs = listify' sh sp" 
+      by fastforce
+  with evf_pushlam have "v = hp \<and> 
+    h' = H (hh(hp := 1, Suc hp := sh sp, Suc (Suc hp) := pc')) (Suc (Suc (Suc hp)))" by fastforce
+  with S have X: "FS h' env (v # vs) (pc # p # sfs) = 
+    restructure (US (hh(hp := 1, Suc hp := p, Suc (Suc hp) := pc')) (3 + hp) e ep 
+      (vs'(vp := hp)) (Suc vp) sh (Suc sp) pc)" by simp
+  from evf_pushlam S have "cd \<tturnstile> US hh hp e ep vs' vp sh (Suc sp) (Suc pc) \<leadsto>\<^sub>u 
+    US (hh(hp := 1, Suc hp := sh sp, Suc (Suc hp) := pc')) (3 + hp) e ep (vs'(vp := hp)) 
+      (Suc vp) sh (Suc sp) pc" by (metis diff_Suc_1 evu_pushlam)
+  with S X show ?case by blast
 next
   case (evf_apply cd pc h v2 p' pc' env v1 env' p2 vs p sfs)
+  then obtain h' hp e ep vs' vp sh sp where S: "\<Sigma>\<^sub>u = US h' hp e ep vs' vp sh (Suc sp) (Suc pc) \<and> 
+    h = H h' hp \<and> env = H e ep \<and> v1 # v2 # vs = listify' vs' vp \<and> p = sh sp \<and> sfs = listify' sh sp" 
+      by fastforce
+
   then show ?case by simp
 next
   case (evf_return cd pc h env vs p sfs)
+  then obtain h' hp e ep vs' vp sh sp where S: "\<Sigma>\<^sub>u = US h' hp e ep vs' vp sh (Suc sp) (Suc pc) \<and> 
+    h = H h' hp \<and> env = H e ep \<and> vs = listify' vs' vp \<and> p = sh sp \<and> sfs = listify' sh sp" 
+      by fastforce
+
   then show ?case by simp
 next
   case (evf_jump cd pc h v2 p' pc' env v1 env' p2 vs p sfs)
+  then obtain h' hp e ep vs' vp sh sp where S: "\<Sigma>\<^sub>u = US h' hp e ep vs' vp sh (Suc sp) (Suc pc) \<and> 
+    h = H h' hp \<and> env = H e ep \<and> v1 # v2 # vs = listify' vs' vp \<and> p = sh sp \<and> sfs = listify' sh sp" 
+      by fastforce
+
   then show ?case by simp
 qed
 
