Compiler.thy
@@ -67,12 +67,12 @@ proof -
     (CES hempty hempty [] [(0, length ?cd)]) \<Sigma>\<^sub>c\<^sub>e' \<and> HS h\<^sub>h [v\<^sub>h] [] = unchain_state \<Sigma>\<^sub>c\<^sub>e'" by fastforce
   then obtain h\<^sub>c\<^sub>e env\<^sub>h where VCE: "\<Sigma>\<^sub>c\<^sub>e' = CES h\<^sub>c\<^sub>e env\<^sub>h [v\<^sub>h] [] \<and> h\<^sub>h = unchain_heap h\<^sub>c\<^sub>e env\<^sub>h" 
     by (metis unchain_state_reverse map_is_Nil_conv unchain_stack_def)
-  with ECE have "iter (\<tturnstile> ?cd \<leadsto>\<^sub>f) (flatten (CES hempty hempty [] [(0, length ?cd)]))
+  have CS: "chained_state (CES hempty hempty [] [(0, length ?cd)])" by simp
+  with ECE VCE have "iter (\<tturnstile> ?cd \<leadsto>\<^sub>f) (flatten (CES hempty hempty [] [(0, length ?cd)]))
     (flatten (CES h\<^sub>c\<^sub>e env\<^sub>h [v\<^sub>h] []))" by (metis completef_iter)
   hence EF: "iter (\<tturnstile> ?cd \<leadsto>\<^sub>f) (FS (H nmem 0) (H nmem 0) [] [length ?cd, 0])
      (FS (flatten_values h\<^sub>c\<^sub>e) (flatten_environment env\<^sub>h) [3 * v\<^sub>h] [])" by (simp add: hempty_def)
-  have "chained_state (CES hempty hempty [] [(0, length ?cd)])" by simp
-  with ECE have "chained_state \<Sigma>\<^sub>c\<^sub>e'" by (metis preserve_chained)
+  with ECE CS have "chained_state \<Sigma>\<^sub>c\<^sub>e'" by (metis preserve_chained)
   with VCE have VH: "hcontains h\<^sub>c\<^sub>e v\<^sub>h" by simp
   from C have "?cd \<noteq> []" by auto
   with EF have "\<exists>\<Sigma>\<^sub>u'. 
@@ -117,7 +117,7 @@ proof -
   with SH have "print_hclosure (hlookup h\<^sub>h v\<^sub>h) = print_nexpr (erase v\<^sub>t)" by simp
   with VCE VH have "print_ceclosure (hlookup h\<^sub>c\<^sub>e v\<^sub>h) = print_nexpr (erase v\<^sub>t)" by (metis print_ce)
   with VH have "print_ceclosure (get_closure (flatten_values h\<^sub>c\<^sub>e) (3 * v\<^sub>h)) = print_nexpr (erase v\<^sub>t)" 
-    by simp
+    by (simp del: get_closure.simps)
   with VU VSU have "print_uval h\<^sub>u (vs\<^sub>u 0) = print_nexpr (erase v\<^sub>t)" by (metis print_u)
   hence PU: "print_uval (?mem Hp) (?mem Val 0) = print_nexpr (erase v\<^sub>t)" by simp
   have "unmap_mem (4 * ?mem Val 0) = (Hp, ?mem Val 0)" by simp
